My solutions for PSet1

pset1/Pset1.v
@@ -16,16 +16,25 @@ Require Import Frap Pset1Sig.
 (* Define [Neg] so that it implements Boolean negation, which flips
  * the truth value of a Boolean value.
  *)
-Definition Neg (b : bool) : bool.
-Admitted.
 
+Print eq.
+Definition Neg (b : bool) : bool :=
+  match b with
+  | true => false
+  | false => true
+  end.
+
+Compute (Neg false).
 (* For instance, the negation of [true] should be [false].
  * This proof should follow from reducing both sides of the equation
  * and observing that they are identical.
  *)
 Theorem Neg_true : Neg true = false.
 Proof.
-Admitted.
+  unfold Neg.
+  Search (?x = ?x).
+  apply eq_refl.
+Qed.
 
 (* Negation should be involutive, meaning that if we negate
  * any Boolean value twice, we should get the original value back. 
@@ -36,39 +45,73 @@ Admitted.
  *)
 Theorem Neg_involutive : forall b : bool, Neg (Neg b) = b.
 Proof.
-Admitted.
+  intro b.
+  cases b.
+  - unfold Neg.
+    apply eq_refl.
+  - unfold Neg.
+    apply eq_refl.
+Qed.
 
 (* Define [And] so that it implements Boolean conjunction. That is,
  * the result value should be [true] exactly when both inputs
  * are [true].
  *)
-Definition And (x y : bool) : bool.
-Admitted.
+Definition And (x y : bool) : bool :=
+  match x, y with
+  | true, true => true 
+  | _, _ => false
+  end.
+
 
 (* Here are a couple of examples of how [And] should act on
  * concrete inputs. 
  *)
 Theorem And_true_true : And true true = true.
 Proof.
-Admitted.
+  unfold And.
+  apply eq_refl.
+Qed.
 
 Theorem And_false_true : And false true = false.
 Proof.
-Admitted.
+  unfold And.
+  apply eq_refl.
+Qed.
+
+Print eq.
 
 (* Prove that [And] is commutative, meaning that switching the order
  * of its arguments doesn't affect the result.
  *)
 Theorem And_comm : forall x y : bool, And x y = And y x.
 Proof.
-Admitted.
+  intros.
+  cases x.
+  - cases y.
+    * unfold And.
+      apply eq_refl.
+    * unfold And.
+      apply eq_refl.
+  - cases y.
+    * unfold And.
+      apply eq_refl.
+    * unfold And.
+      apply eq_refl.
+Qed.
 
 (* Prove that the conjunction of a Boolean value with [true]
  * doesn't change that value.
  *)
 Theorem And_true_r : forall x : bool, And x true = x.
 Proof.
-Admitted.
+  intro x.
+  cases x.
+  - unfold And.
+    apply eq_refl.
+  - unfold And.
+    apply eq_refl.
+Qed.
 
 (* In the second part of this assignment, we will work with a simple language
  * of imperative arithmetic programs that sequentially apply operations
@@ -83,43 +126,74 @@ Print Prog.
  * that running the program [p] should result in, when the
  * initial state is [n].
  *)
-Fixpoint run (p : Prog) (initState : nat) : nat.
-Admitted.
+Fixpoint run (p : Prog) (initState : nat) : nat :=
+  match p with
+  | Done => initState
+  | AddThen n p => run p (initState + n)
+  | MulThen n p => run p (initState * n)
+  | SetToThen n p => run p n
+  end.
+
+Compute (run (AddThen 2 (MulThen 4 Done)) 5).
+
+Compute (run (SetToThen 1 (AddThen 2 (MulThen 4 Done))) 5).
+
+ 
 
 Theorem run_Example1 : run Done 0 = 0.
 Proof.
-Admitted.
+  unfold run.
+  apply eq_refl.
+Qed.
 
 Theorem run_Example2 : run (MulThen 5 (AddThen 2 Done)) 1 = 7.
 Proof.
-Admitted.
+  unfold run.
+  ring.
+Qed.
 
 Theorem run_Example3 : run (SetToThen 3 (MulThen 2 Done)) 10 = 6.
 Proof.
-Admitted.
+  unfold run.
+  ring.
+Qed.
 
 (* Define [numInstructions] to compute the number of instructions
  * in a program, not counting [Done] as an instruction.
  *)
-Fixpoint numInstructions (p : Prog) : nat.
-Admitted.
+Fixpoint numInstructions (p : Prog) : nat :=
+  match p with
+  | Done => 0
+  | AddThen _ p => 1 + numInstructions p
+  | MulThen _ p => 1 + numInstructions p
+  | SetToThen _ p => 1 + numInstructions p 
+  end.
 
 Theorem numInstructions_Example :
   numInstructions (MulThen 5 (AddThen 2 Done)) = 2.
 Proof.
-Admitted.
+  simplify.
+  apply eq_refl.
+Qed.
 
 (* Define [concatProg] such that [concatProg p1 p2] is the program
  * that first runs [p1] and then runs [p2].
  *)
-Fixpoint concatProg (p1 p2 : Prog) : Prog.
-Admitted.
+Fixpoint concatProg (p1 p2 : Prog) : Prog :=
+  match p1 with
+  | Done => p2
+  | AddThen n p => AddThen n (concatProg p p2)
+  | MulThen n p => MulThen n (concatProg p p2)
+  | SetToThen n p => SetToThen n (concatProg p p2)
+  end.
+
 
 Theorem concatProg_Example :
      concatProg (AddThen 1 Done) (MulThen 2 Done)
      = AddThen 1 (MulThen 2 Done).
 Proof.
-Admitted.
+  reflexivity.
+Qed.
 
 (* Prove that the number of instructions in the concatenation of
  * two programs is the sum of the number of instructions in each
@@ -129,7 +203,10 @@ Theorem concatProg_numInstructions
   : forall (p1 p2 : Prog), numInstructions (concatProg p1 p2)
                       = numInstructions p1 + numInstructions p2.
 Proof.
-Admitted.
+  intros.
+  induction p1; reflexivity || cbn; rewrite IHp1; apply eq_refl.
+Qed.
+    
 
 (* Prove that running the concatenation of [p1] with [p2] is
    equivalent to running [p1] and then running [p2] on the
@@ -139,4 +216,5 @@ Theorem concatProg_run
     run (concatProg p1 p2) initState =
     run p2 (run p1 initState).
 Proof.
-Admitted.
+  induction p1; reflexivity || simplify; rewrite IHp1; apply eq_refl.
+Qed.
